

Week 12

Lecture 1

Standard Normal Vector

Let

$$z_1, z_2, \dots, z_d \sim \mathcal{N}(0, 1)$$

be independent standard normal random variables.

Define the random vector

$$z = \begin{bmatrix} z_1 \\ \vdots \\ z_d \end{bmatrix}.$$

Since the components are independent, the joint density is

$$f_Z(z) = \prod_{i=1}^d \frac{1}{\sqrt{2\pi}} \exp\left(-\frac{1}{2} z_i^2\right).$$

Using

$$\sum_{i=1}^d z_i^2 = \|z\|^2,$$

we obtain the compact form

$$f_Z(z) = \frac{1}{(2\pi)^{d/2}} \exp\left(-\frac{1}{2} \|z\|^2\right).$$

Simple Linear Transform of a 2D Standard Normal

Let

$$z = \begin{bmatrix} z_1 \\ z_2 \end{bmatrix}, \quad z_1, z_2 \sim \mathcal{N}(0, 1), \text{ independent.}$$

Define

$$\begin{aligned} x_1 &= z_1, \\ x_2 &= \rho z_1 + \sqrt{1 - \rho^2} z_2, \end{aligned}$$

where $-1 < \rho < 1$.

In matrix form,

$$x = Az,$$

with

$$A = \begin{bmatrix} 1 & 0 \\ \rho & \sqrt{1 - \rho^2} \end{bmatrix}.$$

The inverse is

$$A^{-1} = \begin{bmatrix} 1 & 0 \\ -\frac{\rho}{\sqrt{1 - \rho^2}} & \frac{1}{\sqrt{1 - \rho^2}} \end{bmatrix}.$$

Determinants:

$$\det(A) = \sqrt{1 - \rho^2},$$

$$\det(A^{-1}) = \frac{1}{\sqrt{1 - \rho^2}}.$$

Mean and Covariance

Mean:

$$\mathbb{E}[x_1] = 0, \quad \mathbb{E}[x_2] = 0.$$

Variance:

$$\text{Var}(x_1) = 1,$$

$$\text{Var}(x_2) = \rho^2 + (1 - \rho^2) = 1.$$

Covariance:

$$\text{Cov}(x_1, x_2) = \mathbb{E}[x_1 x_2] = \rho.$$

Covariance matrix:

$$\Sigma = \begin{bmatrix} 1 & \rho \\ \rho & 1 \end{bmatrix}.$$

Observe:

$$\Sigma = AA^\top.$$

Determinant:

$$\det(\Sigma) = 1 - \rho^2.$$

Inverse:

$$\Sigma^{-1} = \frac{1}{1 - \rho^2} \begin{bmatrix} 1 & -\rho \\ -\rho & 1 \end{bmatrix}.$$

Density via Change of Variables

Using change of variables,

$$f_X(x) = f_Z(A^{-1}x) |\det(A^{-1})|.$$

Since

$$f_Z(z) = \frac{1}{2\pi} \exp\left(-\frac{1}{2} \|z\|^2\right),$$

we obtain

$$f_X(x) = \frac{1}{2\pi\sqrt{1 - \rho^2}} \exp\left(-\frac{1}{2} x^\top \Sigma^{-1} x\right).$$

Explicitly,

$$f_X(x_1, x_2) = \frac{1}{2\pi\sqrt{1 - \rho^2}} \exp\left(-\frac{1}{2(1 - \rho^2)} (x_1^2 - 2\rho x_1 x_2 + x_2^2)\right).$$

Factorization and Conditional Distributions

The joint density factorizes as

$$f_{X_1, X_2}(x_1, x_2) = f_{X_1}(x_1) f_{X_2|X_1}(x_2|x_1).$$

Marginal:

$$X_1 \sim \mathcal{N}(0, 1).$$

Conditional:

$$X_2 \mid X_1 = x_1 \sim \mathcal{N}(\rho x_1, 1 - \rho^2).$$

By symmetry,

$$X_2 \sim \mathcal{N}(0, 1),$$

$$X_1 \mid X_2 = x_2 \sim \mathcal{N}(\rho x_2, 1 - \rho^2).$$

General Bivariate Normal

Let

$$x = Az + \mu,$$

where

$$z \sim \mathcal{N}(0, I),$$

and

$$\Sigma = AA^\top.$$

Then

$$x \sim \mathcal{N}(\mu, \Sigma),$$

with density

$$f_X(x) = \frac{1}{2\pi\sqrt{\det(\Sigma)}} \exp\left(-\frac{1}{2}(x - \mu)^\top \Sigma^{-1}(x - \mu)\right).$$

General covariance form:

$$\Sigma = \begin{bmatrix} a^2 & \rho ab \\ \rho ab & b^2 \end{bmatrix},$$

with $a > 0$, $b > 0$, $|\rho| < 1$.

Multivariate Normal in Dimension d

Let

$$x = Az + \mu,$$

where

$$z \sim \mathcal{N}(0, I_d),$$

and

$$\Sigma = AA^\top.$$

Then

$$x \sim \mathcal{N}(\mu, \Sigma),$$

with density

$$f_X(x) = \frac{1}{(2\pi)^{d/2} \sqrt{\det(\Sigma)}} \exp \left(-\frac{1}{2} (x - \mu)^\top \Sigma^{-1} (x - \mu) \right).$$

Mean:

$$\mathbb{E}[x] = \mu.$$

Covariance:

$$\text{Cov}(x) = \Sigma.$$

Important Properties

Let

$$x \sim \mathcal{N}(\mu, \Sigma).$$

Linear Scalar Transform

If

$$y = a^\top x,$$

then

$$y \sim \mathcal{N}(a^\top \mu, a^\top \Sigma a).$$

Linear Vector Transform

If

$$y = Bx,$$

then

$$y \sim \mathcal{N}(B\mu, B\Sigma B^\top).$$

Independence Property

For components x_i and x_j of a multivariate normal:

$$x_i \text{ and } x_j \text{ independent} \iff \Sigma_{ij} = 0.$$

Uncorrelated components of a multivariate normal are independent.

Lecture 2

Parameter Estimation

Let $\mathcal{P} = \{P_\theta : \theta \in \Theta\}$ be a family of probability distributions indexed by parameter θ .

Given data

$$X_1, X_2, \dots, X_n \stackrel{iid}{\sim} P_{\theta_0}$$

for some unknown $\theta_0 \in \Theta$,

Goal: Estimate the true parameter θ_0 from data.

Maximum Likelihood Estimation

Likelihood Function

Given observations x_1, \dots, x_n ,

$$L(\theta) = P(X_1 = x_1, \dots, X_n = x_n \mid \theta)$$

Under independence,

$$L(\theta) = \prod_{i=1}^n f_\theta(x_i)$$

where f_θ denotes the pmf or pdf.

Log-Likelihood

$$\ell(\theta) = \log L(\theta) = \sum_{i=1}^n \log f_\theta(x_i)$$

Negative Log-Likelihood

Define the risk function

$$R(\theta) = -\ell(\theta) = -\sum_{i=1}^n \log f_\theta(x_i)$$

Maximum likelihood estimate

$$\hat{\theta}_{ML} = \arg \max_{\theta} L(\theta) = \arg \max_{\theta} \ell(\theta) = \arg \min_{\theta} R(\theta)$$

Example 1: Bernoulli Bias

Model

$$\mathcal{P} = \{\text{Bern}(\theta) : \theta \in 0, 1\}$$

Data:

$$X_i \in \{0, 1\}$$

pmf

$$P_{\theta}(X = x) = \begin{cases} \theta & x = 1 \\ 1 - \theta & x = 0 \end{cases}$$

Compact form:

$$P_{\theta}(x) = \theta^x (1 - \theta)^{1-x}$$

Negative Log-Likelihood

$$\begin{aligned} R(\theta) &= - \sum_{i=1}^n \log(\theta^{x_i} (1 - \theta)^{1-x_i}) \\ &= - \sum_{i=1}^n (x_i \log \theta + (1 - x_i) \log(1 - \theta)) \end{aligned}$$

Let

$$a = \sum_{i=1}^n x_i$$

Then

$$R(\theta) = a \log \frac{1}{\theta} + (n - a) \log \frac{1}{1 - \theta}$$

Minimization

Setting derivative to zero gives

$$\hat{\theta}_{ML} = \frac{a}{n} = \frac{1}{n} \sum_{i=1}^n x_i$$

Important observation:

ML estimate equals sample mean.

Example 2: Uniform Distribution

Model

$$\mathcal{P} = \{\text{Unif}(a, b) : a, b \in \mathbb{R}, a < b\}$$

Density:

$$f_{\theta}(x) = \begin{cases} \frac{1}{b-a} & x \in [a, b] \\ 0 & \text{otherwise} \end{cases}$$

Equivalent form:

$$f_{\theta}(x) = \frac{1}{b-a} \mathbf{1}(x \in [a, b])$$

Negative Log-Likelihood

$$R(\theta) = - \sum_{i=1}^n \log \left(\frac{1}{b-a} \mathbf{1}(x_i \in [a, b]) \right)$$

If any $x_i \notin [a, b]$, then

$$R(\theta) = \infty$$

Thus require

$$a \leq \min_i x_i, \quad b \geq \max_i x_i$$

Then

$$R(\theta) = n \log(b-a)$$

Minimization

To minimize $n \log(b-a)$, choose smallest interval containing data:

$$\hat{a}_{ML} = \min_i x_i$$

$$\hat{b}_{ML} = \max_i x_i$$

Example 3: Normal Mean, Variance Known

Model

$$\mathcal{P} = \{\mathcal{N}(\mu, 1) : \mu \in \mathbb{R}\}$$

Density:

$$f_{\mu}(x) = \frac{1}{\sqrt{2\pi}} \exp\left(-\frac{1}{2}(x - \mu)^2\right)$$

Negative Log-Likelihood

Ignoring constants independent of μ ,

$$R(\mu) = \sum_{i=1}^n \frac{1}{2}(x_i - \mu)^2 + C$$

First-Order Condition

$$\frac{\partial R}{\partial \mu} = -\sum_{i=1}^n (x_i - \mu)$$

Setting to zero,

$$\sum_{i=1}^n (x_i - \mu) = 0$$

$$\hat{\mu}_{ML} = \frac{1}{n} \sum_{i=1}^n x_i$$

Important observation:

ML estimate equals sample mean.

Example 4: Normal Mean and Variance Unknown

Model

$$\mathcal{P} = \{\mathcal{N}(\mu, \sigma^2) : \mu \in \mathbb{R}, \sigma^2 > 0\}$$

Density:

$$f_{\mu, \sigma^2}(x) = \frac{1}{\sigma\sqrt{2\pi}} \exp\left(-\frac{1}{2} \frac{(x - \mu)^2}{\sigma^2}\right)$$

Negative Log-Likelihood

Ignoring constants:

$$R(\mu, \sigma^2) = \frac{n}{2} \log(\sigma^2) + \frac{1}{2} \sum_{i=1}^n \frac{(x_i - \mu)^2}{\sigma^2}$$

Derivative with Respect to μ

$$\frac{\partial R}{\partial \mu} = \sum_{i=1}^n \frac{x_i - \mu}{\sigma^2}$$

Setting to zero:

$$\hat{\mu}_{ML} = \frac{1}{n} \sum_{i=1}^n x_i$$

Derivative with Respect to σ^2

Rewrite:

$$R = \frac{n}{2} \log(\sigma^2) + \frac{1}{2\sigma^2} \sum_{i=1}^n (x_i - \mu)^2$$

Derivative:

$$\frac{\partial R}{\partial \sigma^2} = \frac{n}{2} \frac{1}{\sigma^2} - \frac{1}{2} \frac{\sum_{i=1}^n (x_i - \mu)^2}{(\sigma^2)^2}$$

Setting to zero:

$$\frac{n}{\sigma^2} = \frac{\sum_{i=1}^n (x_i - \mu)^2}{(\sigma^2)^2}$$

Solving:

$$\hat{\sigma}_{ML}^2 = \frac{1}{n} \sum_{i=1}^n (x_i - \hat{\mu}_{ML})^2$$

Important observation:

ML variance uses denominator n , not $n - 1$.

Extension: Multivariate Normal

Model:

$$\mathcal{P} = \{\mathcal{N}(\mu, \Sigma) : \mu \in \mathbb{R}^d, \Sigma \succ 0\}$$

Data:

$$x_1, \dots, x_N \in \mathbb{R}^d$$

ML estimates:

$$\hat{\mu} = \frac{1}{N} \sum_{i=1}^N x_i$$

$$\hat{\Sigma} = \frac{1}{N} \sum_{i=1}^N (x_i - \hat{\mu})(x_i - \hat{\mu})^T$$

Linear Regression with Gaussian Noise

Model

$$X \in \mathbb{R}^d, \quad Y \in \mathbb{R}$$

$$Y = w^T X + \varepsilon$$

$$\varepsilon \sim \mathcal{N}(0, \sigma^2)$$

Thus,

$$Y \mid X \sim \mathcal{N}(w^T X, \sigma^2)$$

Data:

$$(x_1, y_1), \dots, (x_n, y_n)$$

Likelihood

$$L(w) = \prod_{i=1}^n \frac{1}{\sigma \sqrt{2\pi}} \exp \left(-\frac{1}{2\sigma^2} (y_i - w^T x_i)^2 \right)$$

Negative Log-Likelihood

Ignoring constants:

$$R(w) = \frac{1}{2\sigma^2} \sum_{i=1}^n (y_i - w^T x_i)^2 + C$$

Important observation:

Maximum likelihood estimation reduces to minimizing

$$\sum_{i=1}^n (y_i - w^T x_i)^2$$

Thus ML for linear regression with Gaussian noise is equivalent to least squares.

Lecture 3

Gaussian Mixture Models and Expectation Maximization

Motivation: Multi Modal Data

Consider data generated from K different groups. Each group produces observations following a Gaussian distribution with different parameters.

Example in one dimension with $K = 3$:

Component 1:

Mean -4 , variance 0.5 , weight 0.4

Component 2:

Mean 0 , variance 1 , weight 0.3

Component 3:

Mean 5 , variance 1 , weight 0.3

Observed data exhibits multiple peaks. A single Gaussian cannot model such multi modal behavior.

Definition: Gaussian Mixture Model

Let $X \in \mathbb{R}^d$.

A Gaussian Mixture Model with K components has density

$$f_X(x) = \sum_{k=1}^K \pi_k \mathcal{N}(x \mid \mu_k, \Sigma_k)$$

where

$$\sum_{k=1}^K \pi_k = 1, \quad \pi_k \geq 0$$

and

$$\mathcal{N}(x \mid \mu_k, \Sigma_k) = \frac{1}{(2\pi)^{d/2} |\Sigma_k|^{1/2}} \exp \left(-\frac{1}{2} (x - \mu_k)^T \Sigma_k^{-1} (x - \mu_k) \right)$$

Parameters

For each component k :

Mixing weight π_k

Mean $\mu_k \in \mathbb{R}^d$

Covariance $\Sigma_k \in \mathbb{R}^{d \times d}$

Total parameter set

$$\theta = \{\pi_1, \dots, \pi_K, \mu_1, \dots, \mu_K, \Sigma_1, \dots, \Sigma_K\}$$

Important Observation: Label Non Identifiability

Permutation of component indices does not change the density.

If parameters are swapped between components, the mixture density remains identical.

Latent Variable Formulation

Introduce hidden variable Z .

Definition:

$$P(Z = k) = \pi_k$$

Conditional distribution:

$$X \mid Z = k \sim \mathcal{N}(\mu_k, \Sigma_k)$$

Marginal Distribution

Using marginalization:

$$\begin{aligned} P(X) &= \sum_{k=1}^K P(X, Z = k) \\ &= \sum_{k=1}^K P(X \mid Z = k) P(Z = k) \\ &= \sum_{k=1}^K \pi_k \mathcal{N}(x \mid \mu_k, \Sigma_k) \end{aligned}$$

Thus latent formulation is equivalent to mixture density.

Maximum Likelihood Estimation

Given data

$$\{x_1, x_2, \dots, x_N\}$$

Likelihood:

$$P(\text{Data} \mid \theta) = \prod_{n=1}^N \sum_{k=1}^K \pi_k \mathcal{N}(x_n \mid \mu_k, \Sigma_k)$$

Negative log likelihood:

$$\mathcal{L}(\theta) = - \sum_{n=1}^N \log \left(\sum_{k=1}^K \pi_k \mathcal{N}(x_n \mid \mu_k, \Sigma_k) \right)$$

Direct maximization is difficult because of the summation inside the logarithm.

Chicken and Egg Problem

If component assignments were known:

Parameter estimation reduces to computing sample means and covariances per cluster.

If parameters were known:

Cluster assignments can be inferred probabilistically.

But neither is known.

This motivates the Expectation Maximization algorithm.

E Step: Cluster Responsibilities

Compute posterior probability that point x_n belongs to component k .

Definition:

$$\gamma_{nk} = P(Z = k \mid X = x_n)$$

Using Bayes rule:

$$\gamma_{nk} = \frac{\pi_k \mathcal{N}(x_n \mid \mu_k, \Sigma_k)}{\sum_{j=1}^K \pi_j \mathcal{N}(x_n \mid \mu_j, \Sigma_j)}$$

Properties:

$$\sum_{k=1}^K \gamma_{nk} = 1$$

γ_{nk} is called responsibility of component k for data point n .

Effective Cluster Size

Define

$$N_k = \sum_{n=1}^N \gamma_{nk}$$

Interpreted as soft number of points assigned to component k .

M Step: Parameter Updates

Update means:

$$\mu_k^{new} = \frac{1}{N_k} \sum_{n=1}^N \gamma_{nk} x_n$$

Update covariances:

$$\Sigma_k^{new} = \frac{1}{N_k} \sum_{n=1}^N \gamma_{nk} (x_n - \mu_k^{new})(x_n - \mu_k^{new})^T$$

Update mixing weights:

$$\pi_k^{new} = \frac{N_k}{N}$$

EM Algorithm Summary

1. Initialize parameters π_k, μ_k, Σ_k randomly.
2. E step:
Compute γ_{nk} for all n, k .
3. M step:
Update μ_k, Σ_k, π_k using responsibilities.
4. Repeat E and M steps until convergence.

Conceptual Flow

Latent variable model introduces hidden component index.
Likelihood maximization is difficult due to log of sum structure.
EM alternates between:
Estimating hidden variables using current parameters.
Estimating parameters using expected hidden variables.
This procedure iteratively improves the likelihood.

Application: Clustering

Gaussian mixture models provide probabilistic clustering.
In high dimensional settings, visualization is impossible.
EM based GMM remains a fundamental tool for unsupervised learning.
Gaussian mixture models form a foundational building block in machine learning.

Lecture 4

Tail Bounds and Concentration

Two types of results:

1. Bounds on deviation of a random variable from its mean.
 2. Behavior of averages of many random variables.
-

Markov Inequality

Setup

Let X be a positive random variable such that

$$X \geq 0$$

Let

$$\mathbb{E}[X] = \mu$$

Statement

For any $t > 0$,

$$\mathbb{P}(X \geq t) \leq \frac{\mathbb{E}[X]}{t}$$

Interpretation

If $t < \mu$, then

$$\frac{\mu}{t} > 1$$

and the bound is vacuous since probability is at most 1.

The bound is meaningful for $t \geq \mu$.

Proof

Since $X \geq 0$,

$$\mathbb{E}[X] = \int_0^\infty x f_X(x) dx$$

Split the integral at t :

$$\mathbb{E}[X] = \int_0^t x f_X(x) dx + \int_t^\infty x f_X(x) dx$$

Since $x \geq t$ on $[t, \infty)$,

$$\int_t^\infty x f_X(x) dx \geq \int_t^\infty t f_X(x) dx = t \int_t^\infty f_X(x) dx$$

Thus,

$$\mathbb{E}[X] \geq t \mathbb{P}(X \geq t)$$

Rearranging,

$$\mathbb{P}(X \geq t) \leq \frac{\mathbb{E}[X]}{t}$$

Tightness Example

Let X be discrete:

$$\mathbb{P}(X = 0) = \frac{4}{5}$$

$$\mathbb{P}(X = 50) = \frac{1}{5}$$

Then,

$$\mathbb{E}[X] = \frac{1}{5} \cdot 50 = 10$$

Compute:

$$\mathbb{P}(X \geq 50) = \frac{1}{5}$$

Markov bound:

$$\frac{\mathbb{E}[X]}{50} = \frac{10}{50} = \frac{1}{5}$$

Equality holds.

Chebyshev Inequality

Setup

Let

$$\begin{aligned}\mathbb{E}[X] &= \mu \\ \text{Var}(X) &= \sigma^2\end{aligned}$$

Statement

For any $t > 0$,

$$\mathbb{P}(|X - \mu| \geq t) \leq \frac{\sigma^2}{t^2}$$

Proof via Markov

Observe:

$$|X - \mu| \geq t \iff (X - \mu)^2 \geq t^2$$

Thus,

$$\mathbb{P}(|X - \mu| \geq t) = \mathbb{P}((X - \mu)^2 \geq t^2)$$

Apply Markov to $(X - \mu)^2$:

$$\leq \frac{\mathbb{E}[(X - \mu)^2]}{t^2} = \frac{\text{Var}(X)}{t^2}$$

Sample Mean and Concentration

Let X_1, X_2, \dots, X_n be independent and identically distributed.

Assume

$$\mathbb{E}[X_i] = \mu$$

Define the sample mean:

$$\bar{X}_n = \frac{1}{n} \sum_{i=1}^n X_i$$

Then,

$$\mathbb{E}[\bar{X}_n] = \mu$$

Variance of Sample Mean

Since variables are independent,

$$\text{Var}(\bar{X}_n) = \frac{1}{n^2} \sum_{i=1}^n \text{Var}(X_i) = \frac{1}{n^2} n \sigma^2 = \frac{\sigma^2}{n}$$

Chebyshev Bound for Sample Mean

$$\mathbb{P}(|\bar{X}_n - \mu| \geq \epsilon) \leq \frac{\sigma^2}{n\epsilon^2}$$

Decay rate:

$$O\left(\frac{1}{n}\right)$$

Hoeffding Inequality

Additional Assumption

Assume

$$a \leq X_i \leq b$$

Then,

$$\mathbb{P}(|\bar{X}_n - \mu| \geq \epsilon) \leq 2 \exp\left(-\frac{2n\epsilon^2}{(b-a)^2}\right)$$

Decay rate:

$$O(e^{-n})$$

Exponential decay is much faster than $1/n$.

Convergence Concepts

Convergence in Probability

A sequence X_n converges to X in probability if

$$\lim_{n \rightarrow \infty} \mathbb{P}(|X_n - X| \geq \epsilon) = 0 \quad \forall \epsilon > 0$$

Convergence in Distribution

X_n converges to X in distribution if

$$\lim_{n \rightarrow \infty} F_{X_n}(x) = F_X(x) \quad \forall x$$

Convergence in probability implies convergence in distribution.

Law of Large Numbers

Let X_1, \dots, X_n be iid with

$$\mathbb{E}[X_i] = \mu$$

Define

$$\bar{X}_n = \frac{1}{n} \sum_{i=1}^n X_i$$

Weak Law of Large Numbers

$$\bar{X}_n \rightarrow \mu \quad \text{in probability}$$

Proof Using Chebyshev

If variance is finite,

$$\mathbb{P}(|\bar{X}_n - \mu| \geq \epsilon) \leq \frac{\sigma^2}{n\epsilon^2}$$

As $n \rightarrow \infty$,

$$\frac{\sigma^2}{n\epsilon^2} \rightarrow 0$$

Thus convergence in probability holds.

Central Limit Theorem

Let X_1, X_2, \dots be iid with

$$\begin{aligned}\mathbb{E}[X_i] &= \mu \\ \text{Var}(X_i) &= \sigma^2\end{aligned}$$

Define

$$Y_n = \frac{1}{\sqrt{n}} \sum_{i=1}^n (X_i - \mu)$$

Statement

$$Y_n \rightarrow \mathcal{N}(0, \sigma^2) \quad \text{in distribution}$$

Interpretation

Scaled sums of independent random variables converge to a normal distribution.
This explains ubiquity of the normal distribution in additive phenomena.
Even for moderate n , the approximation is accurate.

Summary of Results

Markov:

$$\mathbb{P}(X \geq t) \leq \frac{\mathbb{E}[X]}{t}$$

Chebyshev:

$$\mathbb{P}(|X - \mu| \geq t) \leq \frac{\sigma^2}{t^2}$$

Hoeffding:

$$\mathbb{P}(|\bar{X}_n - \mu| \geq \epsilon) \leq 2 \exp\left(-\frac{2n\epsilon^2}{(b-a)^2}\right)$$

Weak Law:

$$\overline{X}_n \rightarrow \mu \quad \text{in probability}$$

Central Limit Theorem:

$$\frac{1}{\sqrt{n}} \sum_{i=1}^n (X_i - \mu) \rightarrow \mathcal{N}(0, \sigma^2) \quad \text{in distribution}$$
